extraction/theories/EArities.v
@@ -1,7 +1,7 @@
 
 From Coq Require Import Bool String List Program BinPos Compare_dec Omega.
 From MetaCoq.Template Require Import config utils monad_utils BasicAst AstUtils.
-From MetaCoq.PCUIC Require Import PCUICAst PCUICAstUtils PCUICInduction PCUICTyping PCUICMetaTheory PCUICWcbvEval PCUICLiftSubst PCUICInversion PCUICSR PCUICNormal PCUICSafeReduce PCUICSafeLemmata PCUICSafeChecker PCUICPrincipality PCUICGeneration PCUICSubstitution.
+From MetaCoq.PCUIC Require Import PCUICAst PCUICAstUtils PCUICInduction PCUICTyping PCUICMetaTheory PCUICWcbvEval PCUICLiftSubst PCUICInversion PCUICSR PCUICNormal PCUICSafeReduce PCUICSafeLemmata PCUICSafeChecker PCUICPrincipality PCUICGeneration PCUICSubstitution PCUICElimination.
 From MetaCoq.Extraction Require EAst ELiftSubst ETyping EWcbvEval Extract.
 From Equations Require Import Equations.
 Require Import String.
