extraction/theories/ErasureFunction.v
@@ -1,7 +1,7 @@
 
 From Coq Require Import Bool String List Program BinPos Compare_dec Omega.
 From MetaCoq.Template Require Import config utils monad_utils BasicAst AstUtils.
-From MetaCoq.PCUIC Require Import PCUICAst PCUICAstUtils PCUICInduction PCUICTyping PCUICMetaTheory PCUICWcbvEval PCUICLiftSubst PCUICInversion PCUICConfluence PCUICCumulativity PCUICSR PCUICNormal PCUICSafeReduce PCUICSafeLemmata PCUICSafeChecker PCUICValidity PCUICPrincipality.
+From MetaCoq.PCUIC Require Import PCUICAst PCUICAstUtils PCUICInduction PCUICTyping PCUICMetaTheory PCUICWcbvEval PCUICLiftSubst PCUICInversion PCUICConfluence PCUICCumulativity PCUICSR PCUICNormal PCUICSafeReduce PCUICSafeLemmata PCUICSafeChecker PCUICValidity PCUICPrincipality PCUICElimination.
 From MetaCoq.Extraction Require EAst ELiftSubst ETyping EWcbvEval Extract ExtractionCorrectness.
 From Equations Require Import Equations.
 Require Import String.
