pcuic/theories/PCUICElimination.v
@@ -1,0 +1,202 @@
+(* Distributed under the terms of the MIT license.   *)
+
+From Coq Require Import Bool String List Program BinPos Compare_dec Omega.
+From MetaCoq.Template Require Import config utils monad_utils BasicAst AstUtils.
+From MetaCoq.PCUIC Require Import PCUICTyping PCUICAst PCUICAstUtils PCUICInduction  PCUICWeakening PCUICSubstitution PCUICRetyping PCUICMetaTheory PCUICWcbvEval PCUICSR  PCUICClosed PCUICInversion PCUICGeneration PCUICSafeChecker.
+
+Definition is_prop_sort s :=
+  match Universe.level s with
+  | Some l => Level.is_prop l
+  | None => false
+  end.
+
+Definition Is_proof `{cf : checker_flags} Σ Γ t := ∑ T u, Σ ;;; Γ |- t : T × Σ ;;; Γ |- T : tSort u × is_prop_sort u.
+
+Lemma declared_inductive_inj `{cf : checker_flags} {Σ mdecl mdecl' ind idecl idecl'} :
+  declared_inductive Σ mdecl' ind idecl' ->
+  declared_inductive Σ mdecl ind idecl ->
+  mdecl = mdecl' /\ idecl = idecl'.
+Proof.
+  intros [] []. unfold declared_minductive in *.
+  rewrite H in H1. inversion H1. subst. rewrite H2 in H0. inversion H0. eauto.
+Qed.
+
+Definition Informative`{cf : checker_flags} (Σ : global_env_ext) (ind : inductive) :=
+  forall mdecl idecl,
+    declared_inductive (fst Σ) mdecl ind idecl ->
+    forall Γ args u n (Σ' : global_env_ext),
+      wf Σ' ->
+      PCUICWeakeningEnv.extends Σ Σ' ->
+      Is_proof Σ' Γ (mkApps (tConstruct ind n u) args) ->  
+       #|ind_ctors idecl| <= 1 /\
+       squash (All (Is_proof Σ' Γ) (skipn (ind_npars mdecl) args)).
+
+Lemma elim_restriction_works_kelim1 `{cf : checker_flags} (Σ : global_env_ext) Γ T ind npar p c brs mind idecl : wf Σ ->
+  declared_inductive (fst Σ) mind ind idecl ->
+  Σ ;;; Γ |- tCase (ind, npar) p c brs : T ->
+  (Is_proof Σ Γ (tCase (ind, npar) p c brs) -> False) -> In InType (ind_kelim idecl).
+Proof.
+  intros wfΣ. intros.
+  assert (HT := X).
+  eapply inversion_Case in X as (? & ? & ? & ? & ? & ? & ? & ? & ? & ? & ? & ? & ? & ? & ? & ? & ? & ?). 
+  unfold types_of_case in e0.
+  repeat destruct ?; try congruence. subst. inv e0. 
+  eapply declared_inductive_inj in d as []. 2:exact H. subst.
+  enough (universe_family x6 = InType). rewrite H1 in e1.
+  eapply Exists_exists in e1 as (? & ? & ?). subst. eauto.
+  
+  destruct (universe_family x6) eqn:Eu.
+  - exfalso. eapply H0. exists T. exists x6. split. admit.
+    split. (* 2:{ eapply universe_family_is_prop_sort; eauto. } *)
+    admit. admit.
+  - admit. (* no idea what to do for Set *)
+  - reflexivity.  
+Admitted.                       (* elim_restriction_works *)
+
+
+Lemma elim_restriction_works_kelim2 `{cf : checker_flags} (Σ : global_env_ext) ind mind idecl : wf Σ ->
+  declared_inductive (fst Σ) mind ind idecl ->
+  In InType (ind_kelim idecl) -> Informative Σ ind.
+Proof.
+  intros.
+  destruct (PCUICWeakeningEnv.on_declared_inductive X H) as [[]]; eauto.
+  intros ?. intros. inversion o.
+  eapply declared_inductive_inj in H as []; eauto; subst.
+  clear - onConstructors ind_sorts. try dependent induction onConstructors.
+  (* - cbn. split. omega. econstructor. admit. *)
+  (* -  *)
+Admitted.                       (* elim_restriction_works *)
+
+Lemma elim_restriction_works `{cf : checker_flags} (Σ : global_env_ext) Γ T ind npar p c brs mind idecl : wf Σ ->
+  declared_inductive (fst Σ) mind ind idecl ->
+  Σ ;;; Γ |- tCase (ind, npar) p c brs : T ->
+  (Is_proof Σ Γ (tCase (ind, npar) p c brs) -> False) -> Informative Σ ind.
+Proof.
+  intros. eapply elim_restriction_works_kelim2; eauto.
+  eapply elim_restriction_works_kelim1; eauto.
+Qed.
+
+Lemma declared_projection_projs_nonempty `{cf : checker_flags} {Σ : global_env_ext} { mind ind p a} :
+  wf Σ ->
+  declared_projection Σ mind ind p a ->
+  ind_projs ind <> [].
+Proof.
+  intros. destruct H. destruct H0.
+  destruct (ind_projs ind); try congruence. destruct p.
+  cbn in *. destruct n; inv H0.
+Qed.
+
+Lemma elim_restriction_works_proj_kelim1 `{cf : checker_flags} (Σ : global_env_ext) Γ T p c mind idecl :
+  wf Σ ->
+  declared_inductive (fst Σ) mind (fst (fst p)) idecl ->
+  Σ ;;; Γ |- tProj p c : T ->
+  (Is_proof Σ Γ (tProj p c) -> False) -> In InType (ind_kelim idecl).
+Proof.
+  intros. destruct p. destruct p. cbn in *.
+  eapply inversion_Proj in X0 as (? & ? & ? & ? & ? & ? & ? & ? & ?).
+  destruct x2. cbn in *.
+  pose (d' := d). destruct d' as [? _].
+  eapply declared_inductive_inj in H as []; eauto. subst.
+  pose proof (declared_projection_projs_nonempty X d).
+  eapply PCUICWeakeningEnv.on_declared_projection in d; eauto.
+  destruct d as (? & ? & ?). destruct p.
+  inv o. inv o0.
+  forward onProjections. eauto.
+  inversion onProjections.
+  clear - on_projs_elim. revert on_projs_elim. generalize (ind_kelim x1).
+  intros. induction on_projs_elim; subst.
+  - cbn. eauto.
+  - cbn. right. eauto.  
+Qed. (* elim_restriction_works_proj *)
+
+Lemma elim_restriction_works_proj `{cf : checker_flags} (Σ : global_env_ext) Γ  p c mind idecl T :
+  wf Σ ->
+  declared_inductive (fst Σ) mind (fst (fst p)) idecl ->
+  Σ ;;; Γ |- tProj p c : T ->
+  (Is_proof Σ Γ (tProj p c) -> False) -> Informative Σ (fst (fst p)).
+Proof.
+  intros. eapply elim_restriction_works_kelim2; eauto.
+  eapply elim_restriction_works_proj_kelim1; eauto.
+Qed.                       
+
+Lemma length_of_btys {ind mdecl' idecl' args' u' p pty indctx pctx ps btys} :
+  types_of_case ind mdecl' idecl' (firstn (ind_npars mdecl') args') u' p pty = Some (indctx, pctx, ps, btys) ->
+  #|btys| = #|ind_ctors idecl'|.
+Proof.
+  intros. unfold types_of_case in *.
+  destruct ?; try congruence.
+  destruct ?; try congruence.
+  destruct ?; try congruence.
+  destruct ?; try congruence.
+  destruct ?; try congruence.
+  destruct ?; try congruence. inversion H; subst.  unfold build_branches_type in *.
+  unfold mapi in *.
+  clear - E4. revert btys E4. generalize 0 at 3. induction ((ind_ctors idecl')); cbn; intros.
+  - cbn in E4. inversion E4. subst. reflexivity.
+  - cbn in E4.
+    destruct ?; try congruence.
+    destruct ?; try congruence.
+    destruct ?; try congruence.
+    destruct ?; try congruence.
+    destruct ?; try congruence.
+    destruct ?; try congruence.
+    destruct ?; try congruence.
+    subst. inversion E4. subst. cbn. f_equal.
+    eapply IHl.  eauto.
+Qed.
+
+Lemma tCase_length_branch_inv `{cf : checker_flags} (Σ : global_env_ext) Γ ind npar p n u args brs T m t :
+  wf Σ ->
+  Σ ;;; Γ |- tCase (ind, npar) p (mkApps (tConstruct ind n u) args) brs : T ->
+  nth_error brs n = Some (m, t) ->
+  (#|args| = npar + m)%nat.
+Proof.
+  intros. 
+  eapply inversion_Case in X0 as (? & ? & ? & ? & ? & ? & ? & ? & ? & ? & ? & ? & ? & ? & ? & ? & ? & ?). subst.
+  pose proof (length_of_btys e0).
+  eapply type_mkApps_inv in t1 as (? & ? & [] & ?); eauto.
+  eapply inversion_Construct in t1 as (? & ? & ? & ? & ? & ? & ?); eauto.
+  destruct d0. cbn in *.
+  eapply declared_inductive_inj in d as []; eauto. subst.
+  
+  unfold types_of_case in e0.
+  repeat destruct ?; try congruence. destruct p0, p1; subst. inv E3. inv E1. inv e0.
+  unfold build_branches_type in *.
+  assert (exists t', nth_error x7 n = Some (m, t')).
+  eapply All2_nth_error_Some in H as (? & ?). 2:eassumption. destruct p0.
+  rewrite e. destruct p0. cbn in *. subst. destruct x1. cbn. eauto.
+  destruct H3.
+
+  Lemma map_option_Some X (L : list (option X)) t : map_option_out L = Some t -> All2 (fun x y => x = Some y) L t.
+  Proof.
+    intros. induction L in t, H |- *; cbn in *.
+    - inv H. econstructor.
+    - destruct a. destruct ?. all:inv H. eauto.
+  Qed.
+
+  eapply map_option_Some in E4. 
+  eapply All2_nth_error_Some_r in E4 as (? & ? & ?); eauto. 
+  subst.
+  rewrite nth_error_mapi in e. destruct (nth_error (ind_ctors x11) n) eqn:E7; try now inv e.
+  cbn in e. inv e. destruct p0. destruct p0.
+  cbn in H3.
+  eapply PCUICWeakeningEnv.on_declared_inductive in H1; eauto. destruct H1.
+  depelim o0. cbn in *. unfold on_constructors in *.
+  eapply nth_error_alli in E7; eauto. cbn in E7.
+  depelim E7. cbn in *. destruct s.
+  depelim x2. cbn in *.
+  subst. admit. admit.
+  
+  (* clear - H0 E4. unfold mapi in *. *)
+  (* revert n x7 H0 E4. generalize 0 at 3. induction (ind_ctors x2); intros. *)
+  (* - cbn in E4. inv E4. destruct n0; inv H0. *)
+  (* - cbn in E4. destruct a. destruct ?; try congruence. *)
+  (*   destruct p0. *)
+  (*   destruct ?; try congruence. *)
+  (*   inv E4. destruct ?; try congruence. *)
+  (*   destruct ?; try congruence. *)
+  (*   destruct ?; try congruence. *)
+  (*   inv E. destruct n0; cbn in H0. *)
+  (*   + inversion H0. subst. destruct l. cbn in E0. inv E0. cbn in *. inv H0. *)
+  (*   + eapply IHl in E0. eauto.  *)
+Admitted.                       (* tCase_length_branch_inv *)
